examples/Relations.dfy
@@ -5,11 +5,11 @@
  *  SPDX-License-Identifier: MIT
  *******************************************************************************/
 
-include "../src/Relations.dfy"
+include "../src/dafny/Relations.dfy"
 
 module RelationsExamples {
 
-  import opened Relations
+  import opened Dafny.Relations
 
   lemma BuiltInIntLTIsStrictTotalOrdering()
     ensures StrictTotalOrdering((x: int, y: int) => x < y)
@@ -28,5 +28,50 @@ module RelationsExamples {
 
   lemma BuiltInIntEqIsEquivalenceRelation()
     ensures EquivalenceRelation((x: int, y: int) => (x == y))
+  {}
+
+  lemma BuiltInIntGeIsAntiSymmetricRelation()
+    ensures AntiSymmetric((x: int, y: int) => (x >= y))
+  {}
+
+  lemma BuiltInIntLtIsAsymmetricRelation()
+    ensures Asymmetric((x: int, y: int) => (x < y))
+  {
+  }
+
+  lemma AlwaysTrueIsNotAntiSymmetric()
+    ensures !AntiSymmetric((x: int, y: int) => true)
+  {
+    var f := (x: int, y: int) => true;
+    assert f(2,3) && f(3,2) && 3 != 2;
+    assert !AntiSymmetric(f);
+  }
+
+  lemma BuiltInIntLtIsNotReflexiveRelation()
+    ensures !Reflexive((x: int, y: int) => (x < y))
+  {
+    var f := (x: int, y: int) => (x < y);
+    assert !forall x: int :: f(x,x);
+    assert !Reflexive(f);
+  }
+
+  lemma BuiltInIntLtIsIrreflexiveRelation()
+    ensures Irreflexive((x: int, y: int) => (x < y))
+  {}
+
+  lemma BuiltInIntEqIsNotIrreflexiveRelation()
+    ensures !Irreflexive((x: int, y: int) => (x == y))
+  {
+    var f := (x: int, y: int) => (x == y);
+    assert f(0,0);
+    assert !Irreflexive(f);
+  }
+
+  lemma AsymmetricIsAntiSymmetric<T>(f: (T,T)->bool)
+    ensures Asymmetric(f) ==> AntiSymmetric(f)
+  {}
+
+  lemma AsymmetricIsIrreflexive<T>(f: (T,T)->bool)
+    ensures Asymmetric(f) ==> Irreflexive(f)
   {}
 }
